README.md
@@ -37,15 +37,9 @@ Running `make tests` in the top-level QuickChick folder will check and execute a
 
 ### Documentation
 Yes, we need more! Until then here are some reasonable surrogates:
-  - Catalin's topic proposals for 2015
-    (http://prosecco.gforge.inria.fr/personal/hritcu/students/topics/2015/quick-chick.pdf)
-  - Catalin's presentation at CoqPL 2015 workshop (2015-01-18)
-    (http://prosecco.gforge.inria.fr/personal/hritcu/talks/QuickChick-Verified-Testing-CoqPL.pdf)
-  - Zoe's internship report: A Coq Framework For Verified Property-Based Testing
-    (http://prosecco.gforge.inria.fr/personal/hritcu/publications/verified-testing-report.pdf)
-  - Zoe's thesis defense at NTU Athens (2014-09-08)
-    (http://prosecco.gforge.inria.fr/personal/hritcu/talks/zoe-defense.pdf)
-  - Maxime's presentation at the Coq Workshop (2014-07-18)
-    (http://prosecco.gforge.inria.fr/personal/hritcu/talks/QuickChick-Coq.pdf)
-  - Catalin's presentation at the Coq Working Group @ PPS (2014-03-19)
-    (http://prosecco.gforge.inria.fr/personal/hritcu/talks/QuickChick-PPS.pdf)
+  - Our ITP 2015 submission on [Foundational Property-Based Testing](http://prosecco.gforge.inria.fr/personal/hritcu/publications/foundational-pbt.pdf)
+  - Catalin's [internship topic proposals for 2015](http://prosecco.gforge.inria.fr/personal/hritcu/students/topics/2015/quick-chick.pdf)
+  - Catalin's [presentation at CoqPL 2015 workshop (2015-01-18)](http://prosecco.gforge.inria.fr/personal/hritcu/talks/QuickChick-Verified-Testing-CoqPL.pdf)
+  - Zoe's [thesis defense at NTU Athens (2014-09-08)](http://prosecco.gforge.inria.fr/personal/hritcu/talks/zoe-defense.pdf)
+  - Maxime's [presentation at the Coq Workshop (2014-07-18)](http://prosecco.gforge.inria.fr/personal/hritcu/talks/QuickChick-Coq.pdf)
+  - Catalin's [presentation at the Coq Working Group @ PPS (2014-03-19)](http://prosecco.gforge.inria.fr/personal/hritcu/talks/QuickChick-PPS.pdf)
